\documentclass{article}

\usepackage{amsmath}
\usepackage{amssymb}
\usepackage{amsthm}

\newtheorem{theorem}{Theorem}

\begin{document}

\begin{theorem}
S K K = I.
\end{theorem}


\begin{proof}
$$(\lambda x\;y\;z.x\;z\;(y\;z))\;\underline{(\lambda x\;y.x)\;(\lambda x\;y.x)}\;=\;\lambda x.x$$
{\centering
    \downarrow{\alpha, normal\;strategy}\par
}

$$(\underline{(\lambda x\;y\;z.x\;z\;(y\;z))\;(\lambda x'\;y'.x')})\;(\lambda x''\;y''.x'')\;=\;\lambda x.x$$
{\centering
    \downarrow{\beta}\par
}

$$\underline{(\lambda y\;z.(\lambda x'\;y'.x')\;z\;(y\;z))\;(\lambda x''\;y''.x''})\;=\;\lambda x.x$$
{\centering
    \downarrow{\beta}\par
}

$$\lambda z.(\lambda x'\;y'.x')\;z\;((\lambda x''\;y''.x'')\;z)\;=\;\lambda x.x$$
{\centering
    \downarrow{normal\;strategy}\par
}

$$\lambda z.(\underline{(\lambda x'\;y'.x')\;z})\;((\lambda x''\;y''.x'')\;z)\;=\;\lambda x.x$$
{\centering
    \downarrow{\beta}\par
}

$$\lambda z.\undeline{(\lambda y'.z)\;((\lambda x''\;y''.x'')\;z)}\;=\;\lambda x.x$$
{\centering
    \downarrow{\beta}\par
}

$$\underline{\lambda z.z}\;=\;\lambda x.x$$
{\centering
    \downarrow{\alpha}\par
}

$$\lambda x.x\;=\;\lambda x.x$$
\end{proof}

\end{document}