\documentclass{article}
\begin{document}
{\centering
  Beta-reduction for $((\lambda a.(\lambda b.b\;b)\;(\lambda b.b\;b))\;b)\;((\lambda c.(c\;b))\;(\lambda a.a))$.\par
}

$$(\underline{(\lambda a.(\lambda b.b\;b)\;(\lambda b.b\;b))\;b})\;((\lambda c.(c\;b)) (\lambda a.a))$$
$$\downarrow{\beta}$$

$$((\lambda b.b\;b)\;(\lambda b.b\;b))\;(\underline{(\lambda c.(c\;b)) (\lambda a.a)})$$
$$\downarrow{\beta}$$

$$((\lambda b.b\;b)\;(\lambda b.b\;b))\;(\underline{(\lambda a.a)\;b})$$
$$\downarrow{\beta}$$

$$((\lambda b.b\;b)\;(\lambda b.b\;b))\;b$$

\end{document}